updated the example to implement the allocation of thread identifiers; this example provides another illustration of abstracting ordinary variables by linear variables

Test/civl/Program4.bpl
@@ -1,67 +1,138 @@
 // RUN: %boogie -noinfer -typeEncoding:m -useArrayTheory "%s" > "%t"
 // RUN: %diff "%s.expect" "%t"
-type Tid; 
-var {:layer 0,1} a:[Tid]int;
+var {:layer 0,2} a:[int]int;
+var {:layer 0,1} count: int;
+var {:layer 1,1} {:linear "tid"} unallocated:[int]bool;
 
-procedure {:yields} {:layer 1} main() { 
-    var {:linear "tid"} tid:Tid;
+procedure {:yields} {:layer 2} main()
+requires {:layer 1} AllocInv(count, unallocated);
+{
+    var {:layer 1} {:linear "tid"} tid:int;
+    var i: int;
 
     yield;
-    while (true) { 
-        call tid := Allocate(); 
-	async call P(tid); 
+    assert {:layer 1} AllocInv(count, unallocated);
+    while (true)
+    invariant {:layer 1} AllocInv(count, unallocated);
+    { 
+        call tid, i := Allocate(); 
+	async call P(tid, i); 
 	yield;
+        assert {:layer 1} AllocInv(count, unallocated);	
     }
     yield;
 }
 
-procedure {:yields} {:layer 1} P({:linear "tid"} tid: Tid) 
-ensures {:layer 1} a[tid] == old(a)[tid] + 1; 
+procedure {:yields} {:layer 2} P({:layer 1} {:linear "tid"} tid: int, i: int)
+requires {:layer 1} tid == i;
+requires {:layer 1} AllocInv(count, unallocated);
+ensures {:layer 1} AllocInv(count, unallocated);
+ensures {:layer 2} a[tid] == old(a)[tid] + 1; 
 { 
     var t:int;
 
     yield;
-    assert {:layer 1} a[tid] == old(a)[tid];
-    call t := Read(tid); 
+    assert {:layer 1} AllocInv(count, unallocated);
+    assert {:layer 2} a[tid] == old(a)[tid];
+    call t := Read(tid, i); 
     yield;
-    assert {:layer 1} a[tid] == t; 
-    call Write(tid, t + 1); 
+    assert {:layer 1} AllocInv(count, unallocated);
+    assert {:layer 2} a[tid] == t; 
+    call Write(tid, i, t + 1); 
     yield;
-    assert {:layer 1} a[tid] == t + 1; 
+    assert {:layer 1} AllocInv(count, unallocated);
+    assert {:layer 2} a[tid] == t + 1; 
 }
 
-procedure {:yields} {:layer 1} Allocate() returns ({:linear "tid"} tid: Tid)
+procedure {:yields} {:layer 1,2} Allocate() returns ({:layer 1} {:linear "tid"} tid: int, i: int)
+requires {:layer 1} AllocInv(count, unallocated);
+ensures {:layer 1} AllocInv(count, unallocated);
+ensures {:layer 1} tid == i;
+ensures {:atomic}
+|{A:
+  return true;
+}|;
 {
     yield;
-    call tid := AllocateLow();
+    assert {:layer 1} AllocInv(count, unallocated);
+    call i := AllocateLow();
+    call tid := MakeLinear(i);
     yield;
+    assert {:layer 1} AllocInv(count, unallocated);    
 }
 
-procedure {:yields} {:layer 0,1} Read({:linear "tid"} tid: Tid) returns (val: int);
+procedure {:yields} {:layer 1,2} Read({:layer 1} {:linear "tid"} tid: int, i: int) returns (val: int)
+requires {:layer 1} tid == i;
+requires {:layer 1} AllocInv(count, unallocated);
+ensures {:layer 1} AllocInv(count, unallocated);
 ensures {:atomic}
 |{A:
   val := a[tid]; return true;
 }|;
+{
+    yield;
+    assert {:layer 1} AllocInv(count, unallocated);
+    call val := ReadLow(i);
+    yield;
+    assert {:layer 1} AllocInv(count, unallocated);
+}
 
-procedure {:yields} {:layer 0,1} Write({:linear "tid"} tid: Tid, val: int);
+procedure {:yields} {:layer 1,2} Write({:layer 1} {:linear "tid"} tid: int, i: int, val: int)
+requires {:layer 1} tid == i;
+requires {:layer 1} AllocInv(count, unallocated);
+ensures {:layer 1} AllocInv(count, unallocated);
 ensures {:atomic}
 |{A:
   a[tid] := val; return true;
 }|;
+{
+    yield;
+    assert {:layer 1} AllocInv(count, unallocated);
+    call WriteLow(i, val);
+    yield;
+    assert {:layer 1} AllocInv(count, unallocated);
+}
 
-procedure {:yields} {:layer 0,1} AllocateLow() returns ({:linear "tid"} tid: Tid);
-ensures {:atomic} |{ A: return true; }|;
+function {:inline} AllocInv(count: int, unallocated:[int]bool): (bool)
+{
+    (forall x: int :: count <= x ==> unallocated[x])
+}
 
+procedure {:yields} {:layer 0,1} ReadLow(i: int) returns (val: int);
+ensures {:atomic}
+|{A:
+  val := a[i]; return true;
+}|;
 
+procedure {:yields} {:layer 0,1} WriteLow(i: int, val: int);
+ensures {:atomic}
+|{A:
+  a[i] := val; return true;
+}|;
 
-function {:builtin "MapConst"} MapConstBool(bool): [Tid]bool;
-function {:builtin "MapOr"} MapOr([Tid]bool, [Tid]bool) : [Tid]bool;
+procedure {:yields} {:layer 0,1} AllocateLow() returns (i: int);
+ensures {:atomic}
+|{A:
+  i := count;
+  count := i + 1;
+  return true;
+}|;
 
-function {:inline} {:linear "tid"} TidCollector(x: Tid) : [Tid]bool
+// We can prove that this primitive procedure preserves the permission invariant locally.
+// We only need to using its specification and the definitions of TidCollector and TidSetCollector.
+procedure {:layer 1} MakeLinear(i: int) returns ({:linear "tid"} tid: int);
+requires unallocated[i];
+modifies unallocated;
+ensures tid == i && unallocated == old(unallocated)[i := false];
+
+function {:builtin "MapConst"} MapConstBool(bool): [int]bool;
+function {:builtin "MapOr"} MapOr([int]bool, [int]bool) : [int]bool;
+
+function {:inline} {:linear "tid"} TidCollector(x: int) : [int]bool
 {
   MapConstBool(false)[x := true]
 }
-function {:inline} {:linear "tid"} TidSetCollector(x: [Tid]bool) : [Tid]bool
+function {:inline} {:linear "tid"} TidSetCollector(x: [int]bool) : [int]bool
 {
   x
 }
